theory/Sound_Communication_A.thy
@@ -1873,7 +1873,8 @@ theorem staticOneSyncSound:
 apply (erule staticOneSync.cases; auto)
 apply (unfold one_sync.simps; auto)
 using singular_to_equal
-apply (metis (mono_tags, lifting) forEveryTwo.intros fun_upd_other is_recv_path_implies_nonempty_pool star.refl)
+fan_in.simps fan_out.simps noncompetitive_recv_to_ordered_recv noncompetitive_send_to_ordered_send
+apply(meson star.refl)
 done
 
 end
